Added a new hoisting rewrite relation and proved that the hoisting phase is in the reflexive transitive closure of this relation. Also, added the file relations.v that contains definitions of compatible and reflexive transitive (parametrized by the number of steps) closures of a relation and useful lemmas.

theories/L6_PCPS/hoisting.v
@@ -1,71 +1,173 @@
-Require Import cps cps_util identifiers eval env ctx.
-Require Import List BinNat Relations.
+Require Import cps cps_util identifiers eval env ctx relations.
+Require Import List BinNat Relations Omega.
 
 Import ListNotations.
 
 (* TODO : move dependencies from shrink_cps to common file *)
 
-Fixpoint exp_hoist (e : exp) (defs : fundefs)
+(** Given an expression [e], [exp_hoist e B f] will return an expression [e']
+  * and a block of function definitions [B']. [e'] is the function defintion 
+  * erasure of [e] and [B] is exactly the function definitions of [e]. It's 
+  * writen in a CPS fashion and [f] is the continuation. [B] is an accumulator
+  * of function defitnions. 
+  *)
+Fixpoint erase_fundefs (e : exp) (defs : fundefs)
          (f : exp * fundefs -> exp * fundefs) {struct e} : exp * fundefs :=
   match e with
     | Econstr x typ tag ys e' =>
-      exp_hoist e' defs (fun p => let (e, defs) := p in
-                                  f (Econstr x typ tag ys e, defs))
+      erase_fundefs e' defs (fun p => let (e, defs) := p in
+                                      f (Econstr x typ tag ys e, defs))
     | Ecase x tes =>
       fold_left
         (fun (f : exp * fundefs -> exp * fundefs) (te : tag * exp) =>
            fun p =>
              let (c, e) := te in
              let (e1, defs1) := p in
-             exp_hoist e defs1
+             erase_fundefs e defs1
                        (fun p2 =>
                           let (e2, defs2) := p2 in
                           match e1 with
                             | Ecase x' tes' =>
-                              f (Ecase x' ((c, e2) :: tes), defs2)
+                              f (Ecase x' ((c, e2) :: tes'), defs2)
                             | _ => (* This should never match *)
                               f (Ecase x [(c, e2)], defs2)
-                          end)) tes f (Ecase x tes, defs)
+                          end)) tes f (Ecase x [], defs)
     | Eproj x typ n y e' =>
-      exp_hoist e' defs (fun p =>
+      erase_fundefs e' defs (fun p =>
                            let (e, defs) := p in
                            f (Eproj x typ n y e, defs))
     | Efun fdefs e' =>
-      exp_hoist e' defs (fun p =>
+      erase_fundefs e' defs (fun p =>
                            let (e'', defs'') := p in
-                           fundefs_hoist fdefs e'' defs'' f)
+                           erase_nested_fundefs fdefs e'' defs'' f)
     | Eapp g xs =>
       f (Eapp g xs, defs)
     | Eprim x typ prim ys e' =>
-      exp_hoist e' defs (fun p =>
+      erase_fundefs e' defs (fun p =>
                            let (e', defs') := p in
                            f (Eprim x typ prim ys e', defs'))
   end
-with fundefs_hoist (defs : fundefs) (e : exp) (hdefs : fundefs)
-                   (f : exp * fundefs -> exp * fundefs) {struct defs}
+with erase_nested_fundefs (defs : fundefs) (e : exp) (hdefs : fundefs)
+                          (f : exp * fundefs -> exp * fundefs) {struct defs}
      : exp * fundefs :=
        match defs with 
-         | Fcons g t xs e defs =>
-           fundefs_hoist defs e hdefs
-                         (fun p1 =>
-                            let (e1, defs1) := p1 in
-                            exp_hoist e defs1
-                                      (fun p2 =>
-                                         let (e2, defs2) := p1 in
-                                         (e1, Fcons g t xs e2 defs2)))
+         | Fcons g t xs e' defs =>
+           erase_nested_fundefs defs e hdefs
+                                (fun p1 =>
+                                   let (e1, defs1) := p1 in
+                                   erase_fundefs e' defs1
+                                                 (fun p2 =>
+                                                    let (e2, defs2) := p2 in
+                                                    f (e1, Fcons g t xs e2 defs2)))
          | Fnil => f (e, hdefs)
   end.
 
+(** [exp_hoist e] moves all function definitions of [e] at the outermost level *)
+Definition exp_hoist (e : exp) :=
+  let (e, defs) := erase_fundefs e Fnil id in
+  match defs with
+    | Fnil => e
+    | _ => Efun defs e
+  end.
 
+(** [erase_fundefs e e' B] iff [e'] is [e] after erasing all the function 
+  *  defintion blocks and [B] is exactly the function definitions of [e] 
+  *) 
+Inductive Erase_fundefs : exp -> exp -> fundefs -> Prop :=
+| Efun_erase :
+    forall e e' defs Be Bdefs Be_defs,
+      Erase_fundefs e e' Be ->
+      Erase_nested_fundefs defs Bdefs ->
+      split_fds Be Bdefs Be_defs ->
+      Erase_fundefs (Efun defs e) e' Be_defs
+| Econstr_erase :
+    forall x tau t ys e e' B,
+      Erase_fundefs e e' B ->
+      Erase_fundefs (Econstr x tau t ys e)
+                  (Econstr x tau t ys e') B
+| Ecase_nil_erase :
+    forall x,
+      Erase_fundefs (Ecase x nil) (Ecase x nil) Fnil
+| Ecase_cons_erase :
+    forall x c e e' tes tes' B B' B'',
+      Erase_fundefs (Ecase x tes) (Ecase x tes') B ->
+      Erase_fundefs e e' B' ->
+      split_fds B B' B'' ->
+      Erase_fundefs (Ecase x ((c, e) :: tes)) (Ecase x ((c, e') :: tes')) B''
+| Eproj_erase :
+    forall x tau N y e e' B,
+      Erase_fundefs e e' B ->
+      Erase_fundefs (Eproj x tau N y e)
+                    (Eproj x tau N y e') B
+| Eapp_erase :
+    forall f xs,
+      Erase_fundefs (Eapp f xs) (Eapp f xs) Fnil
+| Eprim_erase :
+    forall x tau f ys e e' B,
+      Erase_fundefs e e' B ->
+      Erase_fundefs (Eprim x tau f ys e)
+                    (Eprim x tau f ys e') B
+with Erase_nested_fundefs : fundefs -> fundefs -> Prop :=
+| Fcons_erase :
+    forall f tau xs e e' defs B B' B'',
+      Erase_fundefs e e' B ->
+      Erase_nested_fundefs defs B' ->
+      split_fds B (Fcons f tau xs e' B') B'' ->
+      Erase_nested_fundefs (Fcons f tau xs e defs) B''
+| Fnil_erase :
+    Erase_nested_fundefs Fnil Fnil.
 
-(** expressions without function definitions *)
+(** Correspondence between the inductive and the computational defintions
+  * of function definition erasure 
+  *)
+Lemma erase_fundefs_in_Erase_fundefs :
+  (forall e B f,
+   exists e' B' B'',
+     erase_fundefs e B f = f (e', B') /\
+     split_fds B B'' B' /\
+     Erase_fundefs e e' B'') /\
+  (forall defs e B f,
+    exists B' B'',
+      erase_nested_fundefs defs e B f = f (e, B') /\
+      split_fds B B'' B' /\
+      Erase_nested_fundefs defs B'').
+Proof.
+  exp_defs_induction IHe IHl IHf; intros; simpl in *;
+  try (now edestruct IHe as [e' [B' [B'' [Heq [Hsplit Her]]]]];
+       repeat eexists; eauto; try rewrite Heq; try constructor; auto).
+  - repeat eexists; eauto using split_fds_nil_l; repeat econstructor.
+  - edestruct IHl as [e1' [B1' [B1'' [Heq1 [Hspl1 Her1]]]]]. 
+    edestruct IHe as [e2' [B2' [B2'' [Heq2 [Hspl2 Her2]]]]].
+    rewrite Heq1, Heq2. clear Heq1 Heq2.
+    edestruct split_fds_trans as [B3 [H1 H2]]; [apply Hspl1 | |]; eauto.
+    inv Her1; repeat eexists; eauto; econstructor; eauto; econstructor; eauto.
+  - edestruct IHe as [e2 [B2 [B2' [Heq2 [Hspl2 Her2]]]]].
+    edestruct IHf as [B1 [B1' [Heq1 [Hspl1 Her1]]]]; subst.
+    edestruct split_fds_trans as [B3 [H1 H2]] ; [ | apply Hspl1 |]; eauto.
+    repeat eexists. rewrite Heq2, Heq1; eauto. eauto. econstructor; eauto.
+  - repeat eexists; eauto using split_fds_nil_l; repeat econstructor.
+  - edestruct IHf as [B1 [B1' [Heq1 [Hspl1 Her1]]]]; subst.
+    edestruct IHe as [e2 [B2 [B2' [Heq2 [Hspl2 Her2]]]]].
+    edestruct split_fds_trans as [B3 [H1 H2]] ; [ apply Hspl1 | |]; eauto.
+    repeat eexists. rewrite Heq1, Heq2; eauto.
+    constructor; eauto. econstructor; eauto. constructor; eauto.
+    apply split_fds_sym; eauto.
+  - repeat eexists; eauto using split_fds_nil_l; repeat econstructor.
+Qed.
+
+(** Expressions without function definitions *)
 Inductive no_fun : exp -> Prop  :=
 | Econstr_no_fun :
     forall x tau t xs e,
       no_fun e ->
       no_fun (Econstr x tau t xs e)
+| Ecase_nil_no_fun :
+    forall x, no_fun (Ecase x [])
 | Ecase_no_fun :
-    forall x txs, no_fun (Ecase x txs)
+    forall x c e tes,
+      no_fun (Ecase x tes) ->
+      no_fun e ->
+      no_fun (Ecase x ((c, e) :: tes))
 | Eproj_no_fun :
     forall x tau n y e,
       no_fun e ->
@@ -75,140 +177,427 @@ Inductive no_fun : exp -> Prop  :=
 | Eprim_no_fun :
     forall x tau p xs e,
       no_fun e ->
-
       no_fun (Eprim x tau p xs e).
 
-(** function definitions without nested function definitions *)
+(** Function definitions without nested function definitions *)
 Inductive no_fun_defs : fundefs -> Prop  :=
 | Fcons_no_fun :
-    forall f tau xs e defs,
+    forall f tau xs e B,
       no_fun e ->
-      no_fun_defs defs ->
-      no_fun_defs (Fcons f tau xs e defs)
+      no_fun_defs B ->
+      no_fun_defs (Fcons f tau xs e B)
 | Fnil_no_fun :
     no_fun_defs Fnil.
 
 Hint Constructors no_fun no_fun_defs.
 
-(** hoisting as a rewrite relation *)
-Inductive hoist_rw : relation exp :=
-| hoist1 :
-    forall e1 e2 defs defs' defs'' e c,
-      split_fds defs defs' defs'' ->
-      no_fun_defs defs' ->
-      app_ctx (Efun1_c defs c) (Efun defs' e) e1 ->
-      app_ctx (Efun1_c defs'' c) e e2 ->
-      hoist_rw e1 e2.
+Lemma no_fun_split_fds B B' B'' :
+  no_fun_defs B -> no_fun_defs B' ->
+  split_fds B B' B'' ->
+  no_fun_defs B''.
+Proof.
+  intros Hnf Hnf' Hsp. induction Hsp; eauto.
+  - inv Hnf; constructor; eauto.
+  - inv Hnf'; constructor; eauto.
+Qed.
 
-(** reflexive transitive closure, parametrized by the 
-    number of steps for induction *)
-Inductive hoist_star_n : nat -> relation exp :=
-| hoistn_step :
-    forall e1 e2 e3 n, hoist_rw e1 e2 ->
-                  hoist_star_n n e2 e3 ->
-                  hoist_star_n (S n) e1 e3
-| hoistn_refl :
-    forall e, hoist_star_n 0 e e.
+
+(** If [Erase_fundefs e e' B] then there are no function defintions 
+    in [e'] and [B] *)
+Lemma erase_fundefs_no_fun :
+  (forall e e' B,
+     Erase_fundefs e e' B ->
+     no_fun e' /\ no_fun_defs B) /\
+  (forall B B',
+     Erase_nested_fundefs B B' ->
+     no_fun_defs B').
+Proof.
+  exp_defs_induction IHe IHl IHf; intros; simpl;
+  try (now inv H; edestruct IHe; eauto);
+  try (now inv H; split; eauto).
+  - inv H. edestruct IHe; eauto.
+    edestruct IHl; eauto. 
+    econstructor. eauto. eapply no_fun_split_fds; [ | | eauto]; eauto.
+  - inv H. edestruct IHe; eauto. split. eauto.
+    eapply no_fun_split_fds; [ | | eauto]; eauto.
+  - inv H. edestruct IHe; eauto. 
+    eapply no_fun_split_fds; [ | | eauto]; eauto.
+  - inv H; eauto.
+Qed.
+
+
+(** Hoisting as a rewrite relation *)
+Inductive hoist_rw : relation exp :=
+| EConstr_hoist :
+    forall x tau t ys B e,
+      hoist_rw (Econstr x tau t ys (Efun B e))
+               (Efun B (Econstr x tau t ys e))
+| Ecase_hoist :
+    forall x tes t e' tes' B,
+      hoist_rw (Ecase x (tes ++ ((t, Efun B e') :: tes')))
+               (Efun B (Ecase x (tes ++ ((t, e') :: tes'))))
+| Eproj_hoist :
+    forall x tau N y e B,
+      hoist_rw (Eproj x tau N y (Efun B e))
+               (Efun B (Eproj x tau N y e))
+| Efun_hoist :
+    forall B B' B'' e,
+      split_fds B B' B'' ->
+      hoist_rw (Efun B (Efun B' e)) (Efun B'' e)
+| Eprim_hoist :
+    forall x tau f ys e B,
+      hoist_rw (Eprim x tau f ys (Efun B e))
+               (Efun B (Eprim x tau f ys e))
+| Fnil_hoist :
+    forall e,
+      hoist_rw (Efun (Fnil) e) e
+| FCons_hoist :
+    forall f tau xs e' e B1 B2 B3 B4 B,
+      split_fds B1 (Fcons f tau xs (Efun B3 e') Fnil) B2 ->
+      split_fds B1 (Fcons f tau xs e' Fnil) B4 ->
+      split_fds B3 B4 B ->
+      hoist_rw (Efun B2 e) (Efun B e).
 
 Definition hoist_star (e1 e2: exp) : Prop :=
-  exists n, hoist_star_n n e1 e2.
+  exists n, refl_trans_closure_n (compat_closure hoist_rw) n e1 e2.
 
-(** Hoisting normal form *)
-Definition hoist_nf (e : exp) :=
-  ~ exists e', hoist_rw e e'.
+(** Number of function definitions in an expression *)
+Fixpoint exp_fun_count (e : exp) : nat :=
+  match e with
+    | Econstr _ _ _ _ e | Eproj _ _ _ _ e
+    | Eprim _ _ _ _ e => exp_fun_count e
+    | Ecase _ P =>
+      fold_left (fun n p => n + (exp_fun_count (snd p))) P 0
+    | Efun B e => exp_fun_count e + fundefs_fun_count B
+    | Eapp _ _ => 0
+  end
+with fundefs_fun_count (B : fundefs) : nat :=
+       match B with
+         | Fcons _ _ _ e B => 1 + exp_fun_count e + fundefs_fun_count B
+         | Fnil => 0
+       end.
 
-
-Definition injective {A B} (f : A -> B) :=
-  forall x y, f x = f y -> x = y.
-
-Lemma injective_comp {A B C} (f : A -> B) (g : B -> C) :
-  injective f -> injective g ->
-  injective (fun x => g (f x)).
+Lemma split_fds_fundefs_fundefs_count B B' B'' :
+  split_fds B B' B'' ->
+  fundefs_fun_count B + fundefs_fun_count B' = fundefs_fun_count B''.
 Proof.
-  unfold injective; eauto.
+  intros H. induction H; eauto; simpl; omega.
 Qed.
 
-(* The following need to be updated.
-
-Lemma exp_fundefs_hoist_no_fun:
-  (forall e,
-   exists g e',
-     (forall defs f,
-        exp_hoist e defs f = Efun (g defs) (f e')) /\
-     injective g /\
-     (forall defs, no_fun_defs defs -> no_fun_defs (g defs)) /\
-     no_fun e') /\
-  (forall defs,
-   exists g,
-     (forall hdefs f,
-        fundefs_hoist defs hdefs f = f (g hdefs)) /\
-     injective g /\
-     forall defs, no_fun_defs defs -> no_fun_defs (g defs)).
+(** The number of functions definitions is invariant w.r.t hoist_rw *)
+Lemma exp_fun_count_invariant n :
+  invariant hoist_rw (fun e => exp_fun_count e = n).
 Proof.
-  exp_defs_induction IHe IHl IHf;
-  intros; try edestruct IHe as [g1 [? [H1 [H2 [H3 H4]]]]];
-  try edestruct IHf as [g2 [H5 [H6 H7]]];
-  try (now do 2 eexists; 
-       simpl; split; [ intros defs f; rewrite H1; eauto | split; eauto ]);
-  try (now exists id; repeat eexists; intros; unfold injective; eauto).
-  simpl. exists (fun x => g1 (g2 x)); eexists.
-  split; intros. rewrite H1, H5; eauto.
-  split; eauto using injective_comp.
-  simpl. exists (fun d => Fcons v t l x (g2 (g1 d))). split.
-  intros; simpl. rewrite H1, H5; eauto. 
-  split; eauto using injective_comp. 
-  eapply injective_comp; eauto using injective_comp.
-  intros x1 x2 Heq; inv Heq; eauto.
+  intros e1 e2 Heq Hrw; inv Hrw; simpl; eauto.
+  - rewrite <- !fold_left_rev_right, !rev_app_distr.
+    simpl. generalize (rev tes') as l', (rev tes) as l, 0.
+    induction l'; intros l n; simpl. omega.
+    rewrite <- IHl'. omega.
+  - erewrite <- split_fds_fundefs_fundefs_count; eauto. omega.
+  - apply split_fds_fundefs_fundefs_count in H.
+    apply split_fds_fundefs_fundefs_count in H0.
+    apply split_fds_fundefs_fundefs_count in H1. simpl in *.
+    omega.
 Qed.
 
-Corollary exp_hoist_head_no_fun e :
-  exists e' g,
-    (forall defs f, exp_hoist e defs f = Efun (g defs) (f e')) /\
-    no_fun e'.
+Lemma fun_count_ctx_compat :
+  (forall c e e', exp_fun_count e = exp_fun_count e' ->
+                  exp_fun_count (c |[ e ]|) = exp_fun_count (c |[ e' ]|)) /\
+  (forall fc e e', exp_fun_count e = exp_fun_count e' ->
+                   fundefs_fun_count (fc <[ e ]>) =
+                   fundefs_fun_count (fc <[ e' ]>)).
 Proof.
-  destruct exp_fundefs_hoist_no_fun as [H1 _].
-  destruct (H1 e) as [? [? H2]]. do 2 eexists.
-  split; eapply H2; eauto.
+  exp_fundefs_ctx_induction IHc IHfc; try now intros e1 e2 Heq; simpl; eauto.
+  simpl. intros l' e1 e2 Heq.
+  rewrite <- !fold_left_rev_right, !rev_app_distr.
+  simpl. generalize (rev l') as l1, (rev l) as l2, 0.
+  induction l1; intros l2 n; simpl.
+  now erewrite IHc; eauto.
+  rewrite IHl1. omega.
 Qed.
 
-Corollary exp_hoist_head e :
-  exists e' g,
-    forall defs f, exp_hoist e defs f = Efun (g defs) (f e').
+(** The number of functions definitions is invariant w.r.t hoist_star *)
+(* TODO : refactor this proof so that it uses the generic lemmas in relations.v *)
+Lemma exp_fun_cnt_refl_trans_clo_invariant m n :
+  invariant (refl_trans_closure_n (compat_closure hoist_rw) m)
+            (fun e => exp_fun_count e = n).
 Proof.
-  destruct exp_fundefs_hoist_no_fun as [H1 _].
-  destruct (H1 e) as [? [? H2]]. do 2 eexists. 
-  intros; eapply H2; eauto.
+  intros e1 e2 H1 Hstar.
+  revert e1 e2 H1 Hstar. induction m; intros e1 e2 H1 Hstar.
+  - inv Hstar. eauto. 
+  - inv Hstar. inv H0. eapply IHm; [| eauto ].
+    apply fun_count_ctx_compat.
+    eapply exp_fun_count_invariant; eauto.
 Qed.
 
-Lemma exp_hoist_f_comp :
-  forall e e' defs hdefs f1 f2,
-    exp_hoist e defs f1 = Efun hdefs (f1 e') ->
-    exp_hoist e defs (fun x => f2 (f1 x)) = Efun hdefs (f2 (f1 e')).
+Lemma hoist_rw_Ecase_cons x c e tes tes' :
+  hoist_rw (Ecase x tes) (Ecase x tes') ->
+  hoist_rw (Ecase x ((c, e) :: tes)) (Ecase x ((c, e) :: tes')).
 Proof.
-  intros e e' defs defs' g g' H.
-  destruct (exp_hoist_head e) as [e'' [g'' H']].
-  rewrite H' in H. inv H.
-  rewrite H'. eauto.
+  intros Hrw. inv Hrw.
+Qed.
+
+Lemma no_fun_Ecase_Efun x tes c B e tes' :
+  ~ (no_fun (Ecase x (tes ++ ((c, Efun B e) :: tes')))).
+Proof.
+  induction tes; simpl; intros Hc; inv Hc; eauto. inv H4.
+Qed.
+  
+Lemma invariant_no_fun :
+  invariant hoist_rw no_fun.
+Proof.
+  intros e1 e2 Hnf Hrw. inv Hnf; inv Hrw; try now inv H.
+  - apply app_eq_nil in H1. inv H1. inv H0.
+  - destruct tes0; simpl in *. inv H3.
+    + inv H0.
+    + inv H3. exfalso. eapply no_fun_Ecase_Efun; eauto.
+Qed.
+
+Lemma ctx_compat_no_fun :
+  ctx_compat no_fun.
+Proof.
+  split.
+  - induction c; simpl; intros e1 e2 Hnf1 Hnf2; inv Hnf1; eauto.
+    + symmetry in H1. apply app_eq_nil in H1. inv H1. inv H0.
+    + revert c0 e tes l0 H1 H2 H0. induction l; intros c0 e tes l0 H1 H2 H0.
+      * simpl in *. inv H0. constructor; eauto.
+      * inv H1.
+        inv H0. symmetry in H3. apply app_eq_nil in H3. inv H3. inv H0.
+        inv H0. simpl. constructor; eauto. 
+  - induction c; simpl; intros e1 Hnf; eauto; try inv Hnf; eauto.
+    + symmetry in H1. apply app_eq_nil in H1. inv H1. inv H0.
+    + revert c0 e tes l0 H1 H2 H0. induction l; intros c0 e tes l0 H1 H2 H0.
+      * inv H0; eauto.
+      * simpl in H0; inv H0. inv H1.
+        symmetry in H3. apply app_eq_nil in H3. inv H3. inv H0.
+        eapply IHl; eauto.
+Qed.
+
+Ltac exp_to_ctx e c :=
+  match e with
+    | Econstr ?x ?tau ?t ?ys ?e => constr:(Econstr_c x tau t ys c)
+    | Ecase ?x (?tes ++ (?t, ?e) :: ?tes') => constr:(Ecase_c x tes t e c tes')
+    | Eproj ?x ?tau ?N ?y ?e => constr:(Eproj_c x tau N y c)
+    | Efun ?B ?e => constr:(Efun1_c B c)
+    | Eprim ?x ?tau ?f ?ys ?e => constr:(Eprim_c x tau f ys c)
+  end.
+
+Fixpoint f c e' e : exp :=
+  match e with
+    | Econstr x tau t ys e =>
+      Econstr x tau t ys (f c e' e)
+    | Ecase x l => Ecase x ((c, e') :: l)
+    | Eproj x tau t y e =>
+      Eproj x tau t y (f c e' e)
+    | Efun B e => Efun B (f c e' e)
+    | Eapp x x0 => e
+    | Eprim x tau f' ys e =>
+      Eprim x tau f' ys (f c e' e)
+  end.
+
+Inductive g (f' : var) (tau' : type) (xs' : list var) (e' : exp)
+: exp -> exp -> Prop :=
+| g_constr :
+    forall x tau t ys e1 e2,
+      g f' tau' xs' e' e1 e2 ->
+      g f' tau' xs' e' (Econstr x tau t ys e1) (Econstr x tau t ys e2)
+| g_proj :
+    forall x tau N y e1 e2,
+      g f' tau' xs' e' e1 e2 ->
+      g f' tau' xs' e' (Eproj x tau N y e1) (Eproj x tau N y e2)
+| g_fun1 :
+    forall B e,
+      B <> Fnil ->
+      g f' tau' xs' e' (Efun B e) (Efun (Fcons f' tau' xs' e' B) e)
+| g_fun2 :
+    forall B e,
+      B <> Fnil ->
+      g f' tau' xs' e' (Efun B e) (Efun B e)
+| g_fun_Fnil :
+    forall e1 e2,
+      g f' tau' xs' e' e1 e2 ->
+      g f' tau' xs' e' (Efun Fnil e1) (Efun Fnil e2)
+| g_prim :
+    forall x tau f ys e1 e2,
+      g f' tau' xs' e' e1 e2 ->
+      g f' tau' xs' e' (Eprim x tau f ys e1) (Eprim x tau f ys e2)
+(* | g_relf : *)
+(*     forall e, g f' tau' xs' e' e e. *)
+| g_app :
+    forall f xs,
+      g f' tau' xs' e' (Eapp f xs) (Eapp f xs)
+ | g_case :
+     forall x P,
+       g f' tau' xs' e' (Ecase x P) (Ecase x P).
+
+
+Lemma hoist_star_Ecase_cons_1 x c e tes tes' :
+  hoist_star (Ecase x tes) (Ecase x tes') ->
+  hoist_star (Ecase x ((c, e) :: tes)) (Ecase x ((c, e) :: tes')).
+Proof.
+  intros [n Hrwstar]. exists n.
+  apply (refl_trans_closure_f_compat (compat_closure hoist_rw) n
+                                     (Ecase x tes) (Ecase x tes')
+                                     (f c e)); eauto.
+  intros e1 e2.
+  apply (compat_closure_f_compat hoist_rw e1 e2 (f c e)); eauto.
+  - intros e1' e2' Hrw; eauto. inv Hrw; simpl; try now constructor.
+    eapply Ecase_hoist with (tes := (c, e) :: tes0).
+    econstructor; eauto.
+  - intros c'. 
+    induction c'; simpl;
+    try (now destruct IHc' as [[c1 Heq] | [c1 Heq]]; [left | right];
+         match goal with
+           | [|- exists c, forall e, ?Ctx (?g (?c' |[ _ ]|))  = _ ]  =>
+             let c := (exp_to_ctx (Ctx (c' |[ e1 ]|)) c1)
+               in exists c 
+                         end; simpl; intros e3; rewrite Heq; eauto).
+    + left. exists Hole_c; eauto.
+    + right. exists (Ecase_c v ((c, e) :: l) t c' l0); eauto.
+    + right. exists (Efun2_c f0 (f c e e0)); eauto.
 Qed.
 
 
-
-Lemma hoist_star_0 :
-  forall e e', hoist_star_n 0 e e' -> e = e'.
+(* This lemma should not be used. Insted we should find a way to use 
+ * the more general lemma compat_closure_g_compat in relations.v *)
+Lemma compat_closure_g_compat (R : relation exp) e1 e2 e1' x tau xs e' :
+  (forall e1 e2 e1', R e1 e2 -> g x tau xs e' e1 e1' ->
+                     exists e2', R e1' e2' /\ g x tau xs e' e2 e2') ->
+  g x tau xs e' e1 e1' ->
+  compat_closure R e1 e2 ->
+  exists e2', compat_closure R e1' e2' /\ g x tau xs e' e2 e2'.
 Proof.
-  assert (H : 0%nat = 0%nat) by reflexivity.
-  revert H. generalize 0%nat at 1 3.
-  intros n  Heq e e' H. induction H; eauto; subst. congruence.
+  intros Hyp Hr' H. inv H.
+  revert e e'0 e' e1' Hyp H0 Hr'.
+  induction c; intros  e3 e4 e1 e2 Hyp H0 Hr'; simpl in *.
+  - edestruct Hyp as [e2'' [Hrw2 Hr2]]; eauto.
+    eexists.  split. apply Compat with (c := Hole_c); eauto. eauto.
+  - inv Hr'. edestruct IHc as [e2'' [Hrw2 Hr2]]; eauto. 
+    eexists; split; eauto.
+    eapply compat_closure_compat with (c:= Econstr_c v t t0 l Hole_c). eauto.
+    constructor. eauto.
+  - inv Hr'. edestruct IHc as [e2'' [Hrw2 Hr2]]; eauto. 
+    eexists; split; eauto.
+    eapply compat_closure_compat with (c:= Eproj_c v t n v0 Hole_c). eauto.
+    constructor. eauto.
+  - inv Hr'. edestruct IHc as [e2'' [Hrw2 Hr2]]; eauto. 
+    eexists; split; eauto.
+    eapply compat_closure_compat with (c:= Eprim_c v t p l Hole_c). eauto.
+    constructor. eauto.
+  - inv Hr'. eexists.  split; try now constructor.
+    apply Compat with (c := Ecase_c v l t c l0); eauto.
+  - inv Hr'.
+    + eexists. split.
+      apply Compat with (c := Efun1_c (Fcons x tau xs e1 f0) c); eauto.
+      constructor; eauto.
+    + eexists. split.
+      apply Compat with (c := Efun1_c f0 c); eauto.
+      constructor; eauto.
+    + edestruct IHc as [e2'' [Hrw2 Hr2]]; eauto.  
+      eexists; split; eauto. 
+      eapply compat_closure_compat with (c:= Efun1_c Fnil Hole_c). eauto.
+      constructor; eauto.
+  -  inv Hr'.
+    + eexists. split.
+      apply Compat with (c := Efun2_c (Fcons2_c x tau xs e1 f0) e); eauto.
+      constructor; eauto. destruct f0; simpl; congruence.
+    + eexists. split.
+      apply Compat with (c := Efun2_c f0 e); eauto.
+      constructor; eauto. destruct f0; simpl; congruence.
+    + destruct f0.  inv H. inv H.
 Qed.
 
-Lemma hoist_star_n_trans n m e1 e2 e3:
-  hoist_star_n n e1 e2 ->
-  hoist_star_n m e2 e3 ->
-  hoist_star_n (n+m) e1 e3.
+Lemma split_fds_Fnil_eq_l B1 B2 :
+  split_fds Fnil B1 B2 -> B1 = B2.
 Proof.
-  intros H1 H2. induction H1; eauto.
-  econstructor 1; eauto.
+  revert B1. induction B2; intros B1 H; auto; inv H; f_equal; eauto.
 Qed.
+
+Lemma split_fds_Fnil_eq_r B1 B2 :
+  split_fds B1 Fnil B2 -> B1 = B2.
+Proof.
+  revert B1. induction B2; intros B1 H; auto; inv H; f_equal; eauto.
+Qed.
+
+Lemma hoist_star_Efun_cons
+      f tau xs e' f1 tau1 xs1 e1' f2 tau2 xs2 e2' B1 B2 e :
+  hoist_star (Efun (Fcons f1 tau1 xs1 e1' B1) e)
+             (Efun (Fcons f2 tau2 xs2 e2' B2) e) ->
+  hoist_star (Efun (Fcons f tau xs e' (Fcons f1 tau1 xs1 e1' B1)) e)
+             (Efun (Fcons f tau xs e' (Fcons f2 tau2 xs2 e2' B2)) e).
+Proof.
+  intros [n Hrwstar]. exists n.
+  edestruct
+    (refl_trans_closure_R_compat (compat_closure hoist_rw) n (g f tau xs e')
+                                 (Efun (Fcons f1 tau1 xs1 e1' B1) e)
+                                 (Efun (Fcons f2 tau2 xs2 e2' B2) e)); simpl; eauto.
+  intros e1 e2 e1'' Hr Hrw.
+  apply (compat_closure_g_compat hoist_rw e1 e2); eauto.
+  - intros e3 e4 e3' Hrw' Hg.
+    inv Hrw'; try (now inv Hg; try inv H5;
+                   eexists; split; constructor; eauto; try (constructor; eauto)).
+    + inv Hg. eexists. split; try now constructor.
+      destruct B. constructor; congruence.
+      apply g_fun_Fnil. constructor.
+    + inv Hg.
+      * eexists; split; eauto.
+        econstructor; constructor; eauto.
+        constructor; eauto using split_fds_Fcons_l.
+      * eexists; split. constructor; eauto.
+        constructor; eauto using split_fds_Fcons_l.
+      * eexists; split. constructor.
+        apply split_fds_Fnil_eq_l in H; subst; eauto.
+    + inv Hg; try congruence.
+      eexists. split; try constructor; eauto.
+    + inv Hg. 
+      * eexists. split. econstructor.
+        econstructor 1. eauto. econstructor 1. eauto.
+        econstructor 2. eauto.
+        constructor. eapply split_fds_Fcons_r; eauto.
+        eapply split_fds_Fcons_r; eauto. congruence.
+      * eexists. split. econstructor; eauto. constructor.
+        do 2 (eapply split_fds_Fcons_r; eauto). congruence.
+      * inv H.
+  - constructor. congruence.
+  - eauto. inv H.  inv H0. eauto. exfalso.
+    eapply exp_fun_cnt_refl_trans_clo_invariant in Hrwstar; eauto.
+    eapply exp_fun_cnt_refl_trans_clo_invariant in H1; eauto.
+    simpl in *. omega.
+Qed.
+
+Lemma hoist_star_Ecase_cons_2 x c e tes tes' B :
+  hoist_star (Ecase x tes) (Efun B (Ecase x tes')) ->
+  hoist_star (Ecase x ((c, e) :: tes)) (Efun B (Ecase x ((c, e) :: tes'))).
+Proof.
+  intros [n Hstar]. exists n. 
+  apply (refl_trans_closure_f_compat (compat_closure hoist_rw) n
+                                     (Ecase x tes) (Efun B (Ecase x tes'))
+                                     (f c e)); eauto.
+  intros e1 e2; eapply (compat_closure_f_compat hoist_rw e1 e2 (f c e)); eauto.
+  - intros e1' e2' Hrw; eauto. inv Hrw; simpl; try now econstructor; eauto.
+    eapply Ecase_hoist with (tes := (c, e) :: tes0).
+  - intros c'. 
+    induction c'; simpl;
+    try (now destruct IHc' as [[c1 Heq] | [c1 Heq]]; [left | right];
+           match goal with
+             | [|- exists c, forall e, ?Ctx (?g (?c' |[ _ ]|))  = _ ]  =>
+               let c := (exp_to_ctx (Ctx (c' |[ e1 ]|)) c1)
+               in exists c 
+           end; simpl; intros e3; rewrite Heq; eauto).
+    + left. exists Hole_c; eauto.
+    + right. exists (Ecase_c v ((c, e) :: l) t c' l0); eauto.
+    + right. exists (Efun2_c f0 (f c e e0)); eauto.
+Qed.
+
+Lemma hoist_star_compat e e' c :
+  hoist_star e e' ->
+  hoist_star (c |[ e ]|) (c |[ e' ]|).
+Proof.
+  intros [n H]. exists n. induction H.
+  - econstructor; eauto. now apply compat_closure_compat.
+  - constructor.
+Qed.
+
 
 Lemma hoist_star_trans e1 e2 e3:
   hoist_star e1 e2 ->
@@ -216,116 +605,184 @@ Lemma hoist_star_trans e1 e2 e3:
   hoist_star e1 e3.
 Proof.
   intros [n H1] [m H2].
-  assert (H := hoist_star_n_trans n m e1 e2 e3 H1 H2).
+  assert (H := refl_trans_closure_n_trans
+                 (compat_closure hoist_rw) n m e1 e2 e3 H1 H2).
   eexists; eauto.
 Qed.
 
-Definition is_exp_ctx_f (f : exp -> exp) :=
-  exists c, forall e, app_ctx_f c e = f e.
-
-Definition is_def_ctx_f (h : exp -> fundefs) :=
-  exists c, forall e, app_f_ctx_f c e = h e.
-
-Definition is_def_ctx_defs (f : fundefs -> fundefs) := 
-  forall h, is_def_ctx_f h -> is_def_ctx_f (fun e => f (h e)).
-
-Lemma is_exp_ctx_f_comp (f1 f2 : exp -> exp) :
-  is_exp_ctx_f f1 -> is_exp_ctx_f f2 ->
-  is_exp_ctx_f (fun x => f1 (f2 x)).
+Lemma Erase_fundefs_Fnil_in_hoist_rw :
+  (forall e e', Erase_fundefs e e' Fnil ->
+                hoist_star e e') /\
+  (forall defs e,
+     Erase_nested_fundefs defs Fnil ->
+     hoist_star (Efun defs e) e).
 Proof.
-  intros [c1 H1] [c2 H2].
-  eexists (comp_ctx_f c1 c2). intros e.
-  rewrite <- app_ctx_f_fuse. rewrite H1. f_equal; eauto.
+  exp_defs_induction IHe IHl IHdefs; intros e' H; inv H.
+  - eapply hoist_star_compat with (c := Econstr_c v t t0 l Hole_c); eauto.
+  - exists 0; econstructor; eauto.
+  - apply split_fds_Fnil in H8. inv H8.
+    specialize (IHl (Ecase v tes') H6). inv IHl; eauto.
+    eapply hoist_star_trans.
+    eapply hoist_star_compat with (c := Ecase_c v [] c Hole_c l); eauto.
+    eapply hoist_star_Ecase_cons_1; try (now eexists; eauto).
+  - eapply hoist_star_compat with (c := Eproj_c v t n v0 Hole_c); eauto.
+  - apply split_fds_Fnil in H6. inv H6.
+    eapply hoist_star_trans.
+    eapply hoist_star_compat with (c := Efun1_c f2 Hole_c); eauto.
+    apply IHdefs; eauto.
+  - exists 0; constructor; eauto.
+  - eapply hoist_star_compat with (c := Eprim_c v t p l Hole_c); eauto.
+  - inv H8.
+  - exists 1. econstructor.
+    apply Compat with (c := Hole_c). constructor.
+    constructor.
 Qed.
 
-Lemma is_def_ctx_f_comp f1 f2 :
-  is_def_ctx_defs f1 -> is_def_ctx_f f2 ->
-  is_def_ctx_f (fun x => f1 (f2 x)).
+Lemma hoist_rw_hoist_star e1 e2 :
+  hoist_rw e1 e2 ->
+  hoist_star e1 e2.
 Proof.
-  eauto.
+  intros H1. eapply hoist_star_trans; eauto.
+  exists 1. econstructor; eauto.
+  apply Compat with (c := Hole_c); eauto.
+  constructor. exists 0; constructor.
 Qed.
 
-Lemma is_exp_ctx_f_defs f e :
-  is_def_ctx_f f -> 
-  is_exp_ctx_f (fun x : exp => Efun (f x) e).
+Lemma Fnil_eq_dec B :
+  B = Fnil \/ B <> Fnil.
 Proof.
-  intros [c1 H1].
-  eexists (Efun2_c c1 e). intros e1. simpl.
-  f_equal; eauto.
+  destruct B; eauto. right; congruence.
 Qed.
 
-(** hoisting is in the reflexive transitive closure of the rewrite relation *)
-Lemma exp_fundefs_hoist_in_hoist_star :
-  (forall e defs f,
-     is_exp_ctx_f f -> 
-     hoist_star (Efun defs (f e)) (exp_hoist e defs f)) /\
-  (forall defs e hdefs f g,
-     (forall d, no_fun_defs d -> no_fun_defs (f d)) ->
-     is_exp_ctx_f g ->
-     is_def_ctx_defs f ->
-     (forall d1 d2 d,
-        split_fds d1 d2 d ->
-        split_fds d1 (f d2) (f d)) ->
-     hoist_star (Efun hdefs (g (Efun (f defs) e)))
-                (Efun (fundefs_hoist defs hdefs f) (g e))).
+Lemma Erase_fundefs_in_hoist_rw :
+  (forall e e' B,
+     B <> Fnil -> Erase_fundefs e e' B ->
+     hoist_star e (Efun B e')) /\
+  (forall B B' e,
+     B' <> Fnil -> Erase_nested_fundefs B B' ->
+     hoist_star (Efun B e) (Efun B' e)).
 Proof.
-  apply exp_def_mutual_ind;
-  [intros x typ tag ys e IHe  fdefs f Hctx | intros x fdefs f Hctx
-   | intros x tes c e IHe IHl fdefs f Hctx
-   | intros x typ n y e IHe fdefs f Hctx | intros defs IHdefs e IHe fdefs f Hctx
-   | intros g xs fdefs f Hctx
-   | intros x  typ pr ys e IHe fdefs f Hctx
-   | intros g typ xs e IHe defs IHdefs e' hdefs f h Hnf Hctx Hctx' Hsp
-   | intros e' hdefs f h Hnf Hctx Hctx' Hsp].
-  - simpl.
-    specialize (IHe fdefs (fun e => f (Econstr x typ tag ys e))).
-    apply IHe.
-    destruct Hctx as [c Hctx].
-    eexists (comp_ctx_f c (Econstr_c x typ tag ys Hole_c)).
-    intros e'. rewrite <- Hctx. now rewrite <- app_ctx_f_fuse. 
-  - eexists. apply hoistn_refl.
-  -  
-
-    - simpl. specialize (IHe fdefs (fun e => f (Eproj x typ n y e))).
-    apply IHe.
-    destruct Hctx as [c Hctx].
-    eexists (comp_ctx_f c (Eproj_c x typ n y Hole_c)).
-    intros e'. rewrite <- Hctx. now rewrite <- app_ctx_f_fuse.
-  - simpl. specialize (IHe (fundefs_hoist defs fdefs id) f).
-    eapply hoist_star_trans; eauto. 
-    specialize (IHdefs e fdefs id f). eapply IHdefs; eauto.
-    unfold is_def_ctx_defs; eauto.
-  - eexists. apply hoistn_refl.
-  - simpl. specialize (IHe fdefs (fun e => f (Eprim x typ pr ys e))).
-    apply IHe.
-    destruct Hctx as [c Hctx].
-    eexists (comp_ctx_f c (Eprim_c x typ pr ys Hole_c)).
-    intros e'. rewrite <- Hctx. now rewrite <- app_ctx_f_fuse.
-  - simpl. destruct (exp_hoist_head_no_fun e) as [e1 [g' [H1 H2]]]. rewrite H1.
-    specialize (IHe hdefs (fun e => h (Efun (f (Fcons g typ xs e defs)) e'))).
-    rewrite H1 in IHe; simpl in *.     
-    specialize
-      (IHdefs e' (g' hdefs) (fun defs => f (Fcons g typ xs e1 defs)) h).
-    simpl in *.
-    eapply hoist_star_trans; [ eapply IHe | eapply IHdefs ]; eauto.
-    apply is_exp_ctx_f_comp; eauto.
-    eapply is_exp_ctx_f_defs with (f := fun x => f (Fcons g typ xs x defs)).
-    eapply Hctx'. exists (Fcons1_c g typ xs Hole_c defs).
-    intros; eauto. intros. 
-    intros g1 [c Hg1]. eapply is_def_ctx_f_comp; eauto.
-    exists (Fcons2_c g typ xs e1 c). intros; simpl; f_equal; eauto.
-    intros d1 d2 d Hds. eapply Hsp. constructor; eauto.
-  - simpl. eexists. econstructor 1; [| econstructor 2].
-    destruct Hctx as [c Hctx].
-    eapply hoist1 with (defs := hdefs) (defs' := f Fnil); eauto.
-    eapply Hsp. apply split_fds_nil_l.
-    apply app_ctx_f_correct. simpl. f_equal; eauto.
-    apply app_ctx_f_correct. simpl. f_equal; eauto.
+  exp_defs_induction IHe IHl IHdefs;
+  [| | | | | | | intros B' e1 Hnil H |intros B' e1 Hnil H ];
+  try intros e1 B' Hnil H; inv H.
+  - eapply hoist_star_trans.
+    eapply hoist_star_compat with (c := Econstr_c v t t0 l Hole_c); eauto.
+    apply hoist_rw_hoist_star. constructor.
+  - congruence.
+  - destruct (Fnil_eq_dec B) as [Heq1 | Heq1];
+    destruct (Fnil_eq_dec B'0) as [Heq2 | Heq2]; subst.
+    + inv H8. congruence.
+    + apply split_fds_Fnil_eq_l in H8; subst.
+      specialize (IHe _ _ Heq2 H7).
+      apply Erase_fundefs_Fnil_in_hoist_rw in H6.
+      eapply hoist_star_trans. 
+      eapply hoist_star_compat with (c := Ecase_c v [] c Hole_c l). eauto.
+      simpl. eapply hoist_star_trans.
+      apply hoist_rw_hoist_star. apply Ecase_hoist with (tes := []).
+      simpl. eapply hoist_star_compat with (c := Efun1_c B' Hole_c).
+      eapply hoist_star_Ecase_cons_1; eauto.
+    + apply split_fds_Fnil_eq_r in H8; subst.
+      specialize (IHl _ _ Heq1 H6).
+      apply Erase_fundefs_Fnil_in_hoist_rw in H7.
+      eapply hoist_star_trans. 
+      eapply hoist_star_compat with (c := Ecase_c v [] c Hole_c l); eauto. 
+      simpl. eapply hoist_star_Ecase_cons_2; eauto.
+    + specialize (IHe _ _ Heq2 H7). specialize (IHl _ _ Heq1 H6).
+      simpl. eapply hoist_star_trans.
+      eapply hoist_star_compat with (c := Ecase_c v [] c Hole_c l); eauto.
+      eapply hoist_star_trans.
+      eapply hoist_star_Ecase_cons_2; eauto.
+      eapply hoist_star_trans.
+      eapply hoist_star_compat with (c := Efun1_c B Hole_c).
+      apply hoist_rw_hoist_star. apply Ecase_hoist with (tes := []).
+      apply hoist_rw_hoist_star. constructor; eauto.
+  - eapply hoist_star_trans.
+    eapply hoist_star_compat with (c := Eproj_c v t n v0 Hole_c); eauto.
+    apply hoist_rw_hoist_star. constructor.
+  - destruct (Fnil_eq_dec Be) as [Heq1 | Heq1];
+    destruct (Fnil_eq_dec Bdefs) as [Heq2 | Heq2]; subst.
+    + inv H6. congruence.
+    + apply split_fds_Fnil_eq_l in H6; subst.
+      specialize (IHdefs _ e Heq2 H3).
+      eapply hoist_star_trans; eauto.
+      eapply hoist_star_compat with (c := Efun1_c B' Hole_c).
+      apply Erase_fundefs_Fnil_in_hoist_rw; eauto.
+    + apply split_fds_Fnil_eq_r in H6; subst.
+      specialize (IHe _ _ Heq1 H2).
+      eapply hoist_star_trans; eauto.
+      apply Erase_fundefs_Fnil_in_hoist_rw; eauto.
+    + specialize (IHe _ _ Heq1 H2). specialize (IHdefs _ e Heq2 H3).
+      eapply hoist_star_trans; eauto.
+      eapply hoist_star_trans.
+      eapply hoist_star_compat with (c := Efun1_c Bdefs Hole_c); eauto.
+      apply hoist_rw_hoist_star. constructor; eauto using split_fds_sym.
+  - congruence.
+  - eapply hoist_star_trans.
+    eapply hoist_star_compat with (c := Eprim_c v t p l Hole_c); eauto.
+    apply hoist_rw_hoist_star. constructor.
+  - destruct (Fnil_eq_dec B'0) as [Heq1 | Heq1]; subst;
+    destruct (Fnil_eq_dec B) as [Heq2 | Heq2]; subst.
+    + eapply hoist_star_trans.
+      eapply hoist_star_compat with (c := Efun2_c (Fcons1_c v t l Hole_c f5) e1); eauto.
+      apply Erase_fundefs_Fnil_in_hoist_rw; eauto. simpl. inv H7. inv H1.
+      inv H8. inv H7. exists 0; constructor.
+    + specialize (IHe _ _ Heq2 H6).
+      eapply hoist_star_trans.
+      eapply hoist_star_compat with (c := Efun2_c (Fcons1_c v t l Hole_c f5) e1); eauto.
+      inv H7. inv H1. simpl.
+      apply hoist_rw_hoist_star.
+      econstructor; try (now constructor 2; apply split_fds_nil_l); eauto.
+    + apply split_fds_Fnil_eq_l in H8; subst.
+      eapply Erase_fundefs_Fnil_in_hoist_rw in H6.
+      specialize (IHdefs _ e1 Heq1 H7).
+      eapply hoist_star_trans.
+      eapply hoist_star_compat with (c := Efun2_c (Fcons1_c v t l Hole_c f5) e1); eauto.
+      simpl. destruct B'0; try congruence. destruct f5; try (inv H7; congruence).
+      apply hoist_star_Efun_cons; eauto. 
+    + specialize (IHdefs _ e1 Heq1 H7). specialize (IHe _ _ Heq2 H6).
+      eapply hoist_star_trans.
+      eapply hoist_star_compat with (c := Efun2_c (Fcons1_c v t l Hole_c f5) e1); eauto.
+      simpl. eapply hoist_star_trans with (e2 := Efun (Fcons v t l (Efun B e') B'0) e1).
+      destruct B'0; try congruence. destruct f5; try (inv H7; congruence).
+      apply hoist_star_Efun_cons; eauto. 
+      apply hoist_rw_hoist_star.
+      econstructor; try (now constructor 2; apply split_fds_nil_l); eauto.
+  - exists 0; constructor.
 Qed.
 
-Open Scope ctx_scope.
-Open Scope env_scope.
+Corollary exp_hoist_in_hoist_star e e' :
+  e' = exp_hoist e ->
+  hoist_star e e'.
+Proof.
+  unfold exp_hoist. destruct (erase_fundefs e Fnil) eqn:Heq.
+  destruct erase_fundefs_in_Erase_fundefs as [H1 _].
+  destruct (H1 e Fnil id)
+    as [e'' [B' [B'' [Heq1 [Heq2 Heq3]]]]]. rewrite Heq in Heq1; inv Heq1.
+  apply split_fds_Fnil_eq_l in Heq2; subst.
+  destruct B'; simpl; intros H; subst.
+  - apply Erase_fundefs_in_hoist_rw; eauto. congruence.
+  - apply Erase_fundefs_Fnil_in_hoist_rw; eauto.
+Qed.
 
+
+(* Is this the expected behavior?
+
+Inductive one_or_many A : Type :=
+| One : A -> one_or_many A
+| Many : (one_or_many A * one_or_many A) -> one_or_many A.
+
+Inductive dummy {A : Type} : one_or_many A -> Prop :=
+| One_dummy :
+    forall a, dummy (One A a) 
+| Two_dummy :
+    forall (p : one_or_many A * one_or_many A),
+      let '(c, e) := p in dummy e ->
+      dummy (Many A p).
+
+*)
+
+
+(* TODO : move the following lemmas to the right files *) 
 Lemma preord_env_permut k x y v1 v2 rho1 rho2 :
   x <> y ->
   preord_env k (M.set x v1 (M.set y v2 rho1)) (M.set x v1 (M.set y v2 rho2)) ->
@@ -380,7 +837,6 @@ Proof.
   intros Hc.  eapply Hin. constructor 2; eauto.
 Qed.
 
-Require Import Omega.
 
 Lemma preord_env_def_funs_permut (k : nat) (f1 f2 : fundefs)
       (rho1 rho2 : env) :
@@ -413,43 +869,3 @@ Proof.
     + edestruct Henv as [v2 [Hget Hpre]]; eauto.
       eexists. rewrite def_funs_neq; eauto. rewrite def_funs_neq; eauto.
 Qed.
-
-
-
-Lemma preord_env_def_funs_weaken (k : nat) (f1 f2 : fundefs)
-      (rho1 rho2 : env) :
-  (forall f, name_in_fundefs f f1 -> ~ name_in_fundefs f f2) ->
-  preord_env k (def_funs f1 f1 rho1 (def_funs f2 f2 rho1 rho1))
-             (def_funs f2 f2 rho2 (def_funs f1 f1 rho2 rho2)) ->
-  preord_env k (def_funs f1 f1 (def_funs f2 f2 rho1 rho1) (def_funs f2 f2 rho1 rho1))
-             (def_funs f2 f2 (def_funs f1 f1 rho2 rho2) (def_funs f1 f1 rho2 rho2)).
-Proof.
-  intros Henv Hname x v Hget. 
-  eapply def_funs_spec in Hget. destruct Hget as [[H1 H2] | [H1 H2]].
-  - eexists. rewrite def_funs_neq; eauto. rewrite def_funs_eq; eauto.
-    split; eauto. inv H2.
-    rewrite preord_val_eq. intros vs1 vs2 j t1 xs1 e1 rho1'' Hlen Hdef Heq.
-    edestruct (setlist_length (def_funs f1 f1 (def_funs f2 f2 rho1 rho1)
-                                        (def_funs f2 f2 rho1 rho1))
-                              (def_funs f1 f1 rho2 rho2)) as [rho2'' Hset]; eauto.
-    do 4 eexists; repeat split; eauto. intros Hlt Hall. admit.
-    (* eapply preord_exp_refl. *)
-    (* eapply preord_env_setlist_l. eapply preord_env_def_funs. *)
-    (* eapply preord_env_monotonic; [| eauto]. omega. eauto. eauto. eauto. *)
-  - eapply def_funs_spec in H2.
-    destruct H2 as [[H3 H4] | [H3 H4]]; subst.
-    + eexists. rewrite def_funs_eq; eauto. split; eauto.
-      rewrite preord_val_eq. intros vs1 vs2 j t1 xs1 e1 rho1' Hlen Hdef Heq.
-      edestruct (setlist_length (def_funs f2 f2 rho1 rho1)
-                                (def_funs f2 f2 (def_funs f1 f1 rho2 rho2)
-                                          (def_funs f1 f1 rho2 rho2))) as [rho2' Hset]; eauto.
-      do 4 eexists; repeat split; eauto. intros Hlt Hall.
-      eapply preord_exp_refl. 
-      eapply preord_env_setlist_l; eauto. eapply preord_env_def_funs.
-      eapply preord_env_monotonic; [| eauto]. omega. eauto. eauto. eauto.
-    + edestruct Henv as [v2 [Hget Hpre]]; eauto.
-      eexists. rewrite def_funs_neq; eauto. rewrite def_funs_neq; eauto.
-  Qed.
-
-        
- *)   
