theories/L6_PCPS/relations.v
@@ -1,0 +1,194 @@
+Require Import Relations.
+Require Import cps ctx.
+
+Section Relations.
+
+  Variable (R : relation exp).
+
+  Open Scope ctx_scope.
+  
+  Inductive compat_closure : relation exp :=
+  | Compat :
+      forall c e e',
+        R e e' ->
+        compat_closure (c |[ e ]|) (c |[ e' ]|).
+      
+  Inductive refl_trans_closure_n : nat -> relation exp :=
+  | Trans :
+      forall n e1 e2 e3,
+        R e1 e2 ->
+        refl_trans_closure_n n e2 e3 ->
+        refl_trans_closure_n (S n) e1 e3
+  | Refl :
+      forall e, refl_trans_closure_n 0 e e.
+
+  Definition invariant (R : relation exp) (I : exp -> Prop)  : Prop :=
+    forall (e1 e2 : exp),
+      I e1 -> R e1 e2 -> I e2.
+
+  Lemma invariant_refl_trans_closure (I : exp -> Prop) n :
+    invariant R I ->
+    invariant (refl_trans_closure_n n) I.
+  Proof.
+    induction n.
+    - intros HInv e1 e2 HI Hrw. inv Hrw; eauto.
+    - intros HInv e1 e2 HI Hrw. inv Hrw.
+      apply (IHn HInv e3 e2); eauto.
+  Qed.
+
+  Definition ctx_compat (I : exp -> Prop) : Prop :=
+    (forall c e e', I (c |[ e ]|) -> I e' ->  I (c |[ e' ]|)) /\
+    (forall c e,  I (c |[ e ]|) ->  I e).
+  
+
+  Lemma invariant_compat_closure (I : exp -> Prop) :
+    invariant R I ->
+    ctx_compat I ->
+    invariant compat_closure I.
+  Proof.
+    intros HInv [HS1 HS2] e1 e2 HI Hrw. inv Hrw.
+    eapply HS1; eauto.
+  Qed.
+
+  Lemma refl_trans_closure_f_compat n e1 e2 f :
+    (forall e1 e2, R e1 e2 -> R (f e1) (f e2)) ->
+    refl_trans_closure_n n e1 e2 ->
+    refl_trans_closure_n n (f e1) (f e2).
+  Proof.
+    revert e1 e2 f. induction n; intros e1 e2 f Hyp H.
+    - inv H. constructor.
+    - inv H. econstructor. apply Hyp. eauto. eauto. 
+  Qed.
+
+  Lemma refl_trans_closure_f_compat_inv n I e1 e2 f :
+    invariant R I ->
+    (forall e1 e2, I e1 -> R e1 e2 -> R (f e1) (f e2)) ->
+    I e1 ->
+    refl_trans_closure_n n e1 e2 ->
+    refl_trans_closure_n n (f e1) (f e2).
+  Proof.
+    intros Inv.
+    revert e1 e2 f. induction n; intros e1 e2 f Hyp Hyp' H.
+    - inv H. constructor.
+    - inv H. econstructor. apply Hyp. eauto. eauto. 
+      apply IHn; eauto.
+  Qed.
+
+  Lemma refl_trans_closure_R_compat n (R' : relation exp) e1 e2 e1' :
+    (forall e1 e2 e1',
+       R' e1 e1' -> R e1 e2 ->
+       exists e2', R e1' e2' /\ R' e2 e2') ->
+    R' e1 e1' -> 
+    refl_trans_closure_n n e1 e2 ->
+    exists e2',
+      R' e2 e2' /\
+      refl_trans_closure_n n e1' e2'.
+  Proof.
+    revert e1 e2 e1'. induction n; intros e1 e2 e1' Hyp Hr1 H.
+    - inv H. exists e1'. constructor; eauto. constructor.
+    - inv H. edestruct Hyp as [e3' [Hrw' Hr3]]; eauto.
+      edestruct IHn as [e2' [Hrw Hr2]]; [ | | eauto |]; eauto.
+      eexists. split; eauto. econstructor; eauto.
+  Qed.
+
+  Lemma refl_trans_closure_R_compat_inv n I (R' : relation exp) e1 e2 e1' :
+    invariant R I ->
+    (forall e1 e2 e1',
+       I e1 -> R' e1 e1' -> R e1 e2 ->
+       exists e2', R e1' e2' /\ R' e2 e2') ->
+    I e1 ->
+    R' e1 e1' -> 
+    refl_trans_closure_n n e1 e2 ->
+    exists e2',
+      R' e2 e2' /\
+      refl_trans_closure_n n e1' e2'.
+  Proof.
+    intros Inv.
+    revert e1 e2 e1'. induction n; intros e1 e2 e1' Hyp Hyp' Hr1 H.
+    - inv H. exists e1'. constructor; eauto. constructor.
+    - inv H.
+      edestruct Hyp as [e3' [Hrw' Hr3]]; eauto.
+      edestruct IHn as [e2' [Hrw Hr2]]; [ | | | eauto |]; eauto.
+      eexists. split; eauto. econstructor; eauto.
+  Qed.
+
+
+  Lemma compat_closure_f_compat e1 e2 f :
+    (forall e1 e2, R e1 e2 -> R (f e1) (f e2)) ->
+    (forall c,  (exists c1, forall e, f (c |[ e ]|) = c1 |[ f e ]|) \/
+                (exists c1, forall e, f (c |[ e ]|) = c1 |[ e ]|)) ->
+    compat_closure e1 e2 ->
+    compat_closure (f e1) (f e2).
+  Proof.
+    intros Hyp1 Hyp2 H. inv H.
+    destruct (Hyp2 c) as [[c' Heq] | [c' Heq]]; rewrite !Heq; econstructor; eauto.
+  Qed.
+
+  Lemma compat_closure_f_compat_inv I e1 e2 f :
+    invariant R I -> ctx_compat I ->
+    (forall e1 e2, I e1 -> R e1 e2 -> R (f e1) (f e2)) ->
+    (forall c,  (exists c1, forall e, f (c |[ e ]|) = c1 |[ f e ]|) \/
+                (exists c1, forall e, f (c |[ e ]|) = c1 |[ e ]|)) ->
+    I e1 ->
+    compat_closure e1 e2 ->
+    compat_closure (f e1) (f e2).
+  Proof.
+    intros Inv [HC1 HC2] Hyp1 Hyp2 HI H. inv H.
+    destruct (Hyp2 c) as [[c' Heq] | [c' Heq]]; rewrite !Heq; econstructor; eauto.
+  Qed.
+
+(* (* How to call these two ?? *)
+Definition rel_ctx_1 c (R : relation exp) :=
+  exists c',
+    (forall e e', R e e' -> R (c |[ e ]|) (c' |[ e' ]|)) /\ 
+    (forall e e', R (c |[ e ]|) e' ->
+                  exists e'', e' = c' |[ e'' ]| /\ R e e'').
+
+ Definition rel_ctx_2 c (R : relation exp) :=
+  exists c',
+    (forall e, R (c |[ e ]|) (c' |[ e ]|)) /\ 
+    (forall e e',
+       R (c |[ e ]|) e' ->
+       (exists e'', e' = c' |[ e'' ]| /\ R e e'') \/ (e' = c' |[ e ]|)).
+ 
+           
+Lemma compat_closure_R_compat I (R R' : relation exp) e1 e2 e1':
+  invariant R I -> ctx_compat I ->
+  (forall e1 e2 e1',
+     I e1 -> R e1 e2 -> R' e1 e1' ->
+     exists e2', R e1' e2' /\ R' e2 e2') ->
+  (forall c, rel_ctx_1 c R' \/ rel_ctx_2 c R') ->
+  I e1 ->
+  R' e1 e1' ->
+  compat_closure R e1 e2 ->
+  exists e2', compat_closure R e1' e2' /\ R' e2 e2'.
+Proof.
+  intros Inv [HC1 HC2] Hyp1 Hyp2 HI Hr1 H. inv H.
+  destruct (Hyp2 c) as [[c' [Hc1 Hc2]] | [c' [Hc1 Hc2]]].
+  - destruct (Hc2 _ _ Hr1)  as [e1'' [Heq1 Hr1']]; subst.
+    edestruct Hyp1 as [e2'' [Heq2 Hr2']]; subst.
+    eapply HC2; eauto. eauto. eauto.
+    eexists; split; eauto. constructor. eauto.
+  - eapply Hc2 in Hr1. inv Hr1.
+    + destruct H as [e'' [Heq Hr]]; subst.
+      edestruct Hyp1 as [e2'' [Heq2 Hr2']]; subst.
+Abort. *)
+
+  Lemma refl_trans_closure_n_trans n m e1 e2 e3:
+    refl_trans_closure_n n e1 e2 ->
+    refl_trans_closure_n m e2 e3 ->
+    refl_trans_closure_n (n+m) e1 e3.
+  Proof.
+    intros H1 H2. induction H1; eauto.
+    econstructor 1; eauto.
+  Qed.
+
+  Lemma compat_closure_compat e1 e2 c :
+    compat_closure e1 e2 ->
+    compat_closure (c |[ e1 ]|) (c |[ e2 ]|).
+  Proof.
+    intros H. inv H. rewrite !app_ctx_f_fuse.
+    constructor; eauto.
+  Qed.
+  
+End Relations.
